WIP serialize raw cbor

src/cbor/raw/pulse/everparse/CBOR.Pulse.Raw.Serialize.fst
@@ -9,14 +9,84 @@ open LowParse.Pulse.Base
 
 open CBOR.Pulse.Raw.Match
 module LP = LowParse.Pulse.Combinators
+module LPI = LowParse.Pulse.Int
+
+inline_for_extraction
+let write_initial_byte_t' : l2r_leaf_writer serialize_initial_byte_t =
+  l2r_leaf_writer_ext
+    (LP.l2r_leaf_write_synth'
+      (LowParse.Pulse.BitSum.l2r_write_bitsum'
+        mk_synth_initial_byte
+        (LPI.l2r_leaf_write_u8 ())
+      )
+      synth_initial_byte
+      synth_initial_byte_recip
+    )
+    _
+
+inline_for_extraction
+let write_long_argument_8_simple_value
+  (b: initial_byte)
+  (sq1: squash ((b.additional_info = additional_info_long_argument_8_bits) == true))
+  (sq2: squash ((b.major_type = cbor_major_type_simple_value) == true))
+: Tot (l2r_leaf_writer (serialize_long_argument b))
+=
+          l2r_leaf_writer_ext
+            (LP.l2r_leaf_write_synth'
+              (LP.l2r_leaf_write_filter
+                (LPI.l2r_leaf_write_u8 ())
+                simple_value_long_argument_wf
+              )
+              (LongArgumentSimpleValue #b ())
+              (LongArgumentSimpleValue?.v)
+            )
+            (serialize_long_argument b)
+
+(* etc. *)
+
+assume val write_header : l2r_leaf_writer serialize_header
+
+module SZ = FStar.SizeT
+module PM = Pulse.Lib.SeqMatch
+module A = Pulse.Lib.Array
+module S = Pulse.Lib.Slice
+
+let nlist_match_array
+  (#t': Type0)
+  (#t: Type)
+  (vmatch: (t' -> t -> slprop))
+  (n: nat)
+  (p: perm)
+  (a: A.array t')
+  (l: LowParse.Spec.VCList.nlist n t)
+: Tot slprop
+= exists* c .
+    A.pts_to a #p c **
+    PM.seq_list_match c l vmatch
+
+assume val l2r_write_nlist_as_array
+  (#t': Type0)
+  (#t: Type)
+  (vmatch: (t' -> t -> slprop))
+  (#k: Ghost.erased parser_kind)
+  (#p: parser k t)
+  (#s: serializer p)
+  (w: l2r_writer vmatch s { k.parser_kind_subkind == Some LP.ParserStrong })
+  (n: SZ.t)
+  (p: perm)
+: l2r_writer (nlist_match_array vmatch (SZ.v n) p) (LowParse.Spec.VCList.serialize_nlist (SZ.v n) s)
+
+assume val ser_body_for_array
+  (f: (p: perm) -> LP.l2r_writer (cbor_match p) serialize_raw_data_item)
+  (p: perm)
+  (c: cbor_raw { CBOR_Case_Array? c })
+  (r: Ghost.erased raw_data_item)
+: LP.l2r_writer_for (cbor_match p) serialize_raw_data_item c r
 
 assume val ser_body
   (f: (p: perm) -> LP.l2r_writer (cbor_match p) serialize_raw_data_item)
   (p: perm)
 : LP.l2r_writer (cbor_match p) serialize_raw_data_item
-
-module S = Pulse.Lib.Slice
-module SZ = FStar.SizeT
 
 let ser_pre
   (p: perm)
